coq-osiris/theories/program_logic/handler_rules.v
@@ -138,7 +138,7 @@ Local Ltac ewp_invert :=
   | |- context [environments.Esnoc _ ?Hwp (ewp_def _ (ret _) _ _)] =>
       iPoseProof (ewp_ret_inv with "[$]") as "HΦ"
   (* EWP crash *)
-  | |- context [environments.Esnoc _ ?Hwp (ewp_def _ (Crash _) _ _)] =>
+  | |- context [environments.Esnoc _ ?Hwp (ewp_def _ (Crash) _ _)] =>
       iMod (ewp_crash_inv with "[$]") as "HΦ"
   end.
 
